src/proof/controllers/statefulset/delete_pod.v
@@ -64,7 +64,7 @@ Lemma wp_deletePod γ model_l pod_l
       "Hown_spec" ∷ own_spec_frag γ (PodV.key stored_pod)
         stored_pod.(PodV.ObjectMeta').(ObjectMetaV.UID') 1
         (ObjectSpecV.PodSpec stored_pod.(PodV.Spec')) ∗
-      "Hreservation" ∷ own_occupied_reserved_frag γ (PodV.key stored_pod)
+      "Hreservation" ∷ own_occupied_reserved_frag γ 1 (PodV.key stored_pod)
         stored_pod.(PodV.ObjectMeta').(ObjectMetaV.UID') ∗
       "Hown_children" ∷ own_children_frag γ parent_key parent_uid 1 children ∗
       "Hown_terminating_children_frag" ∷ own_terminating_children_frag γ parent_key parent_uid phase
